WIP commit, various tweaks

Bound.dfy
@@ -3,18 +3,55 @@ include "Ownership-Recursive.dfy"
 
 type Bound = Owner
 
-
 predicate myBoundsOK(oo : Owner, mb : Bound)
  //basic defiintin: my flattened boumd must be outside any owners bound(s)
 //  { (forall o <- oo :: o.AMFB >= flatten(mb)) }
-    { (forall o <- oo :: flatten(mb) <= o.AMFB) }
+//bnst so far    { (forall o <- oo :: flatten(mb) <= o.AMFB) }
+//next trial
+ {
+  && (flatten(oo) >= flatten(mb))
+//  && (forall o <- oo ::( ((o.AMFB) >= flatten(mb))))
+   && (forall o <- oo ::( (o.AMFX > {}) ==> ((o.AMFB+{o}) >= flatten(mb))))
+  }
 
+predicate subBound(o : Object, mb : Bound)
+  {
+//     (o.AMFX > {}) ==> ((o.AMFB+{o}) >= flatten(mb))
+     (o.AMFX > {}) ==> ((o.AMFB) >= flatten(mb))
+  }
+//  ensures (whole.AMFO > {}) ==> ({part}+part.AMFB)   <= ({whole}+whole.AMFB)
+//  ensures (whole.AMFO > {}) ==> ({whole}+whole.AMFB) >= ({part}+part.AMFB)
+
+
+lemma boundSanity(part : Object, whole : Object, po : Object)
+ decreases part.AMFO
+  requires part.Ready() && whole.Ready()
+  requires strictlyInside(part,whole)
+  requires myBoundsOK(part.owner, part.bound)
+   ensures part.AMFO > part.AMFB
+   ensures whole.AMFO > whole.AMFB
+
+  requires po in part.owner
+   ensures po.Ready()
+   ensures (part.owner == {po}) ==> (po.AMFO >= po.AMFB)
+   ensures (part.owner == {po}) ==> (flatten(part.owner) == po.AMFO)
+   ensures (part.owner == {po}) ==> (flatten(part.owner) >= flatten(part.bound))
+   ensures (flatten(part.owner) >= flatten(part.bound))
+   ensures (part.owner == {po}) ==> (po.AMFX > {}) ==> ((po.AMFB+{po}) >= flatten(part.bound))
+   ensures (part.owner == {po}) ==> (po.AMFX > {}) ==> (flatten(part.bound)) <= (po.AMFB+{po})
+   ensures subBound(po, part.bound)
+
+//   ensures (whole.AMFO > {}) ==> (whole.AMFB > {})
+{}
+
+//next trial
 // && (flatten(oo) >= flatten(mb)) //aka effectiveowner is INSIDE effectivebound
 // && (forall o <- oo :: o.AMFB >= flatten(mb))
 
 lemma testBounds1(oo : Owner, mb : Bound)
   //bound of {} is always OK
  requires AllReady(oo)
+ requires AllReady(mb)
   ensures myBoundsOK(oo, {})
   {}
 
@@ -25,13 +62,16 @@ lemma testBounds3(oo : Owner, mb : Bound)
 
 lemma testBounds4(oo : Owner, mb : Bound)
  //kinda just repeats the defn
+  requires flatten(oo) >= flatten(mb)
   requires AllReady(oo)
-  requires forall o <- oo :: o.AMFB >= flatten(mb)
+  requires AllReady(mb)
+  requires forall o <- oo :: o.AMFB+{o} >= flatten(mb)   //PLUSo
    ensures myBoundsOK(oo, mb)
   {}
 
 lemma  {:isolate_assertions} {:timeLimit 20} testBounds5(oo : Owner, mb : Bound)
   requires AllReady(oo)
+  requires flatten(oo) >= flatten(mb)
   requires forall o <- oo :: (o.bound == o.owner)
    ensures forall o <- oo :: (o.AMFB == o.AMFX)
   requires forall o <- oo :: o.AMFX >= flatten(mb)
@@ -68,28 +108,26 @@ lemma testBounds10(oo : Owner, mb : Bound)
   {}
 
 lemma testBounds11(oo : Owner, mb : Bound)
+    requires flatten(oo) >= flatten(mb)
     requires AllReady(oo)
-    requires forall b <- flatten(mb), o <- oo :: b in o.AMFB
-     ensures forall o <- oo :: o.AMFB >= flatten(mb)
+    requires forall b <- flatten(mb), o <- oo :: b in o.AMFB+{o} //PLUSo
+     ensures forall o <- oo :: (o.AMFB+{o}) >= flatten(mb)   ///how come no PLUSo????
+     ensures(forall o <- oo :: ((o.AMFX > {}) ==> ((o.AMFB+{o}) >= flatten(mb))))
      ensures myBoundsOK(oo, mb)
   {}
 
 
 
-lemma   {:isolate_assertions} {:timeLimit 20}  testBounds12(oo : Owner, mb : Bound)
+lemma   {:isolate_assertions} {:timeLimit 20}  testBounds12(oo : Owner, mb : Bound)    //BROKENl
+    requires flatten(oo) >= flatten(mb)
     requires AllReady(oo)
 //    requires mb == (set o <- oo | forall b <- mb :: inside(b,o))
 //    requires mb == (set o <- flatten(oo) | forall b <- flatten(mb) :: inside(b,o))
-    requires mb == (set o <- oo | forall b <- o.AMFB:: inside(o,b))
-
-  // ensures forall o <- oo :: o.AMFB >= flatten(mb)
-     // ensures myBoundsOK(oo, mb)
+//    requires mb == (set o <- oo | forall b <- o.AMFB :: inside(o,b))
+//    requires mb == (set o <- oo | forall b <- o.AMFB+{o} :: inside(o,b))
+//    ensures forall o <- oo :: (o.AMFB+{o}) >= flatten(mb)
+//    ensures myBoundsOK(oo, mb)
   { }
-
-//    mb == (set o <- oo | forall b <- mb :: inside(b,o))
-//
-//
-// lemma {:isolate_assertions} {:timeLimit 20}  testIntersets
 
 
 lemma testBounds13(a : Object, b : Object, c : Object, d : Object)
@@ -106,7 +144,9 @@ lemma testBounds13(a : Object, b : Object, c : Object, d : Object)
 lemma testBounds14(a : Object, b : Object, c : Object, d : Object)
 //simple row
      requires c.AMFB == {a}
+     requires c.AMFO == {c,b,a}
      requires b.AMFB == {a}
+     requires b.AMFO == {a,b}
      requires a.AMFB == {}
      requires a.AMFO == {a}
       ensures myBoundsOK( {c,b}, {a})
@@ -119,7 +159,9 @@ lemma testBounds14(a : Object, b : Object, c : Object, d : Object)
 lemma testBounds15(a : Object, b : Object, c : Object, d : Object)
 //simple row
      requires c.AMFB == {b,a}
+     requires c.AMFO == {b,a,c}
      requires b.AMFB == {a}
+     requires b.AMFO == {b,a}
      requires a.AMFB == {}
      requires a.AMFX == {}
      requires a.Ready()
@@ -132,6 +174,11 @@ lemma testBounds15(a : Object, b : Object, c : Object, d : Object)
         // assert c.AMFB >= flatten({a});
       }
 
+
+
+//////////////////////////////////////////////////////////////////////
+////////
+/////// note all these proposedBNounds doesn't indlude the PLUSo
 
 method proposeBoundsFLAT(os : set<Object>) returns (b : Bound)
  //computes the intersection of the *flattened* bounds of each owner
@@ -163,36 +210,94 @@ method opposeBounds(os : set<Object>) returns (b : Bound)
     set a <- all | forall o <- os :: a in o.AMFB
  }
 
+
  function froposeBounds(os : set<Object>) : (b : Bound)
  //propose boubnsf but it;'s a function withtout READY as a precondition.
- //  ensures myBoundsOK(os, b)
+//   ensures myBoundsOK(os, b)
  {
     var all : set<Object> := set o <- os, a <- o.bound :: a;
-    set a <- all | forall o <- os :: a in o.AMFB
+    set a <- all | forall o <- os :: a in (o.AMFB)
  }
 
-lemma froposeGetsBoundsOK(os : set<Object>, fp  : set<Object>)
+lemma {:isolate_assertions} froposeGetsBoundsOK(os : set<Object>, fp  : set<Object>)
     requires froposeBounds(os) == fp
     requires AllReady(os)
+     ensures froposeBounds(os) == fp
      ensures proposeBounds(os) == fp
+
      ensures myBoundsOK(os, fp)
 {}
 
 
-lemma {:isolate_assertions} TransitiveBounds(part : Object,  whole : Object)
+//////////////////////////////////////////////////////////////////////
+
+lemma {:isolate_assertions} {:timeLimit 30} TransitiveBounds(part : Object,  whole : Object)
  decreases part.AMFO
   requires part.Ready() && whole.Ready()
   requires inside(part,whole)
-  requires myBoundsOK(part.owner, part.bound)
-   ensures part.AMFB <= whole.AMFB //contravariuant
+  requires SingleOwnership(part)
+   ensures SingleOwnership(whole)
+   ensures myBoundsOK(part.owner, part.bound)
+   // ensures part.AMFB <= whole.AMFB //contravariuant
+   // ensures (whole.AMFO > {}) ==> (part.AMFB) <= (whole.AMFB) //contravariuant
+  ensures forall o <- whole.owner ::( (o.AMFX > {}) ==> ((o.AMFB+{o}) >= flatten(whole.bound)))
   {
      InsideRecInside2(part, whole);
+     assert myBoundsOK(part.owner, part.bound);
+       assert (flatten(part.owner) >= flatten(part.bound));
+       assert (forall o <- part.owner ::( (o.AMFX > {}) ==> ((o.AMFB+{o}) >= flatten(part.bound))));
 
     if  ((part == whole) || (whole in part.owner)) { return; }
+
+assert part.AMFO > {};
 
     assert (exists x <- part.owner :: recInside(x,whole));
 
     var next :| ((next in part.owner) && recInside(next,whole));
     InsideRecInside1(next, whole);
-    TransitiveBounds(next,whole);
+assert next in part.owner;
+assert SingleOwnership(part);
+assert |part.owner| == 1;
+LemmaIsSingleton(part.owner);
+assert forall x <- part.owner :: x == next;
+assert (part.owner == {next}); //SingleOwnership
+assert (forall o <- part.owner ::((o.AMFX > {}) ==> ((o.AMFB+{o}) >= flatten(part.bound))));
+
+//// //// //// //// //// //// //// //// //// //// //// //// //// //// //// //// ////
+    assert next.Ready();
+    assert myBoundsOK(next.owner, next.bound);
+
+    assert (flatten(next.owner) >= flatten(next.bound));
+    assert (flatten(part.owner) >= flatten(part.bound));
+
+    assert (forall o <- next.owner ::( (o.AMFX > {}) ==> ((o.AMFB+{o}) >= flatten(next.bound))));
+//  {
+//   && (flatten(oo) >= flatten(mb))
+//   && (forall o <- oo ::( (o.AMFX > {}) ==> ((o.AMFB+{o}) >= flatten(mb))))
+//   }
+//// //// //// //// //// //// //// //// //// //// //// //// //// //// //// //// ////
+
+   TransitiveBounds(next,whole);
 }
+
+
+lemma OneIsOne(n : Object, nn : set<Object>)
+  requires n in nn
+  requires |nn| == 1
+   ensures exists x :: x in nn
+   ensures forall y <- nn, z <- nn :: y == z
+   ensures forall z <- nn :: z == n
+   ensures nn == {n}
+ {
+  LemmaIsSingleton(nn);
+ }
+
+
+
+predicate {:isolate_assertions} SingleOwnership(o : Object)
+  requires o.Ready()
+ decreases o.AMFO
+  {
+    && ((|o.owner| < 2))
+    && ((|o.owner| == 1) ==> (forall oo <- o.owner :: SingleOwnership(oo)))
+  }
